wip: notations, step, todo.md

theories/pl.v
@@ -2,20 +2,22 @@ From Stdlib Require Import Nat.
 From Stdlib Require Import List.
 Import ListNotations.
 
+Module SLang.
+
 (** Variáveis e Labels *)
 
 Inductive variable : Type :=
-  | X : nat -> variable  (* input *)
-  | Z : nat -> variable  (* local *)
-  | Y : variable.
-
+  | X : nat -> variable  (* input  *)
+  | Z : nat -> variable  (* local  *)
+  | Y : variable.        (* output *)
 Inductive label : Type :=
   | A : nat -> label.
 
 Inductive statement : Type :=
   | INCR : variable -> statement
   | DECR : variable -> statement
-  | IF   : variable -> label -> statement.
+  | IF   : variable -> label -> statement
+  | SKIP : variable -> statement.
 
 Inductive instruction : Type :=
   | L_instr : label -> statement -> instruction
@@ -23,7 +25,42 @@ Inductive instruction : Type :=
 
 Definition program := list instruction.
 
+Definition eqb_var v1 v2 := 
+  match v1, v2 with 
+  | X a, X b => a =? b
+  | Z a, Z b => a =? b
+  | Y, Y  => true
+  | _, _ => false
+  end.
+
+Theorem eqb_var_refl : forall v, eqb_var v v = true.
+Proof.
+  destruct v; try (apply PeanoNat.Nat.eqb_refl); reflexivity.
+Qed.
+
+Theorem var_eqb_eq : forall v1 v2 : variable, eqb_var v1 v2 = true <-> v1 = v2.
+Proof.
+  intros v1 v2. split; intros H.
+  (* -> *) 
+  destruct v1; destruct v2; (try discriminate).
+  - simpl in H. rewrite PeanoNat.Nat.eqb_eq in H. rewrite H. reflexivity.
+  - simpl in H. rewrite PeanoNat.Nat.eqb_eq in H. rewrite H. reflexivity.
+  - reflexivity.
+  (* <- *)
+  - rewrite H. apply eqb_var_refl.
+Qed.
+
+Theorem var_eqb_neq : forall v1 v2 : variable, eqb_var v1 v2 = false <-> v1 <> v2.
+Proof.
+  intros v1 v2. split; intros H.
+  - intros H1. rewrite H1 in H. rewrite eqb_var_refl in H. discriminate.
+  - unfold not in H. destruct (eqb_var v1 v2) eqn:Heq.
+    + apply var_eqb_eq in Heq. contradiction. 
+    + reflexivity.
+Qed.
+
 (** Notações adaptadas de: https://softwarefoundations.cis.upenn.edu/lf-current/Imp.html *)
+(* TODO: Aprender... *)
 
 Declare Custom Entry com.
 Declare Scope com_scope.
@@ -36,8 +73,14 @@ Notation "x" := x (in custom com at level 0, x constr at level 0) : com_scope.
 
 Notation "x <- + 1" := (INCR x)
   (in custom com at level 50, left associativity).
+
 Notation "x <- - 1" := (DECR x)
   (in custom com at level 50, left associativity).
+
+Notation "x <- + 0" := (SKIP x)
+  (in custom com at level 50, left associativity).
+
+
 Notation "'IF' x 'GOTO' y " :=
          (IF x y) 
            (in custom com at level 89, x at level 99,
@@ -58,16 +101,61 @@ Open Scope com_scope.
 
 (** Exemplos *)
 
+
+
 Definition x := X 0.
 Definition x1 := X 1.
 Definition l := A 0.
 Definition y := Y.
 
-Check (<{x <- + 1}>).
+Check (instr (INCR (X 0))).
+
+(* Check ([ ] (X 0) <- + 1). *)
 
 
 Definition prg : program :=
   <{[ [l] x  <- + 1;
-      [ ] x1 <- - 1;
+      [ ] x  <- - 1;
+      [ ] x  <- + 0;
       [ ] IF x GOTO l ]}>.
 
+(** Estado de um Programa *)
+(* Referências: 
+  https://softwarefoundations.cis.upenn.edu/lf-current/Maps.html
+  https://github.com/gustavovzqz/coq-lambda/blob/main/theories/Lambda.v
+*)
+
+Definition state := variable -> nat.
+
+Definition initial_state : state := (fun _ => 0).
+
+Definition t_update (m : state ) (x : variable) (v : nat) :=
+  fun x' => if eqb_var x x' then v else m x'.
+
+Definition t_incr (m : state ) (x : variable) :=
+  let v := m x in 
+  fun x' => if eqb_var x x' then (v + 1) else m x'.
+
+Definition t_decr (m : state ) (x : variable) :=
+  let v := m x in 
+  fun x' => if eqb_var x x' then (v - 1) else m x'.
+
+Inductive step : program -> (nat * state) -> (nat * state) -> Prop :=
+  | S_Incr : forall p x i m l ins,
+      nth_error p i = Some ins ->
+      (ins = instr (INCR x) \/ ins = L_instr l (INCR x)) ->
+      step p (i, m) (i + 1, t_incr m x)
+
+  | S_Decr : forall p x i m l ins,
+      nth_error p i = Some ins ->
+      (ins = instr (DECR x) \/ ins = L_instr l (DECR x)) ->
+      step p (i, m) (i + 1, t_decr m x)
+
+  | S_Skip : forall p x i m l ins,
+      nth_error p i = Some ins ->
+      (ins = instr (SKIP x) \/ ins = L_instr l (SKIP x)) ->
+      step p (i, m) (i + 1, m).
+
+(* Completar... *)
+
+End SLang.
